src/tls/MITLS.Repr.ClientHello.fst
@@ -1,0 +1,51 @@
+module MITLS.Repr.ClientHello
+module LP = LowParse.Low.Base
+module B = LowStar.Monotonic.Buffer
+module HS = FStar.HyperStack
+module R = MITLS.Repr
+module CH = Parsers.ClientHello
+open FStar.Integers
+open FStar.HyperStack.ST
+
+let repr #p #q (b:LP.slice p q) =
+  R.repr_p CH.clientHello b CH.clientHello_parser
+
+let meta #p #q (b:LP.slice p q) (from to:R.index b) (h:HS.mem)
+  : Pure (Ghost.erased (R.repr_meta CH.clientHello))
+    (requires
+      R.valid_pos b CH.clientHello_parser from to h)
+    (ensures fun m ->
+      let open R in
+      let r = { start_pos = from;
+                end_pos = to;
+                meta = m } in
+      valid r h)
+  = let open R in
+    let v = LP.contents CH.clientHello_parser h b from in
+    Ghost.hide ({
+      parser_kind = _;
+      parser = CH.clientHello_parser;
+      value = v
+    })
+
+let mk #p #q (b:LP.slice p q) (from to:R.index b)
+  : Stack (repr b)
+    (requires R.valid_pos b CH.clientHello_parser from to)
+    (ensures fun h0 r h1 ->
+      B.modifies B.loc_none h0 h1 /\
+      R.valid r h1)
+  = let open R in
+    let h = get () in
+    let m = meta b from to h in
+    { start_pos = from;
+      end_pos = to;
+      meta = m }
+
+let version (#b:LP.slice 'p 'q) (r:repr b)
+  : Stack Parsers.ProtocolVersion.protocolVersion
+    (requires R.valid r)
+    (ensures fun h0 _ h1 ->
+      B.modifies B.loc_none h0 h1) //underspecifying the returned value, until we figure out how much we need
+  = let open R in
+    let pos = CH.accessor_clientHello_version b r.start_pos in
+    Parsers.ProtocolVersion.protocolVersion_reader b pos
