src/tls/MITLS.Repr.Handshake.fst
@@ -1,0 +1,63 @@
+module MITLS.Repr.Handshake
+module LP = LowParse.Low.Base
+module B = LowStar.Monotonic.Buffer
+module HS = FStar.HyperStack
+module R = MITLS.Repr
+module HSM = Parsers.Handshake
+module RCH = MITLS.Repr.ClientHello
+module RSH = MITLS.Repr.ServerHello
+open FStar.Integers
+open FStar.HyperStack.ST
+
+let repr #p #q (b:LP.slice p q) =
+  R.repr_p HSM.handshake b HSM.handshake_parser
+
+let handshakeType (#b:LP.slice 'p 'q) (r:repr b)
+  : Stack Parsers.HandshakeType.handshakeType
+    (requires
+      R.valid r)
+    (ensures fun h0 _ h1 ->
+      B.modifies B.loc_none h0 h1)
+  = let open R in
+    let open Parsers.HandshakeType in
+    handshakeType_reader b r.start_pos
+
+let clientHello (#b:LP.slice 'p 'q) (r:repr b)
+  : Stack (option (RCH.repr b))
+    (requires
+      R.valid r)
+    (ensures fun h0 ch h1 ->
+      B.modifies B.loc_none h0 h1 /\
+      (Some? ch ==> R.valid (Some?.v ch) h1))
+  = let open R in
+    let open Parsers.HandshakeType in
+    let tag = handshakeType_reader b r.start_pos in
+    match tag with
+    | Client_hello ->
+      let h = get () in
+      let pos' = HSM.handshake_accessor_client_hello b r.start_pos in
+      assume (LP.valid Parsers.ClientHello.clientHello_parser h b pos');
+      let end_pos = Parsers.ClientHello.clientHello_jumper b pos' in
+      let ch_repr = RCH.mk b pos' end_pos in
+      Some ch_repr
+    | _ -> None
+
+let serverHello (#b:LP.slice 'p 'q) (r:repr b)
+  : Stack (option (RSH.repr b))
+    (requires
+      R.valid r)
+    (ensures fun h0 sh h1 ->
+      B.modifies B.loc_none h0 h1 /\
+      (Some? sh ==> R.valid (Some?.v sh) h1))
+  = let open R in
+    let open Parsers.HandshakeType in
+    let tag = handshakeType_reader b r.start_pos in
+    match tag with
+    | Server_hello ->
+      let h = get () in
+      let pos' = HSM.handshake_accessor_server_hello b r.start_pos in
+      assume (LP.valid Parsers.ServerHello.serverHello_parser h b pos');
+      let end_pos = Parsers.ServerHello.serverHello_jumper b pos' in
+      let sh_repr = RSH.mk b pos' end_pos in
+      Some sh_repr
+    | _ -> None
