src/tls/MITLS.Repr.fst
@@ -1,0 +1,53 @@
+module MITLS.Repr
+module LP = LowParse.Low.Base
+module B = LowStar.Monotonic.Buffer
+module HS = FStar.HyperStack
+open FStar.Integers
+
+let index (b:LP.slice 'p 'q) = i:uint_32{ i <= LP.(b.len) }
+
+noeq
+type repr_meta (t:Type) = {
+  parser_kind: (k:LP.parser_kind{LP.(k.parser_kind_subkind == Some ParserStrong)});
+  parser:LP.parser parser_kind t; //erased anyway
+  value: t;
+}
+
+noeq
+type repr #p #q (t:Type) (b:LP.slice p q) = {
+  start_pos: index b;
+  end_pos: i:index b {start_pos <= i };
+  meta: Ghost.erased (repr_meta t)
+}
+
+let repr_p #p #q (t:Type) (b:LP.slice p q) #k (parser:LP.parser k t) =
+  r:repr t b {
+    let meta = Ghost.reveal r.meta in
+    meta.parser_kind == k /\
+    meta.parser == parser
+  }
+
+let valid_pos #t #p #q (b:LP.slice p q) #k (parser:LP.parser k t) (from to:uint_32) (h:HS.mem) =
+    LP.live_slice h b /\
+    LP.valid_pos parser h b from to
+
+let valid #t #p #q (#b:LP.slice p q) (r:repr t b) (h:HS.mem)
+  : Type
+  = let m = Ghost.reveal r.meta in
+    valid_pos b m.parser r.start_pos r.end_pos h /\
+    m.value == LP.contents m.parser h b r.start_pos
+
+let fp #t #p #q (#b:LP.slice p q) (r:repr t b) =
+  LP.loc_slice_from_to b r.start_pos r.end_pos
+  
+let frame_valid #t #p #q (#b:LP.slice p q) (r:repr t b) (l:B.loc) (h0 h1:HS.mem)
+  : Lemma 
+    (requires 
+      valid r h0 /\
+      B.modifies l h0 h1 /\
+      B.loc_disjoint (fp r) l)
+    (ensures
+      valid r h1)
+    [SMTPat (valid r h1);
+     SMTPat (B.modifies l h0 h1)]
+  = B.modifies_buffer_from_to_elim LP.(b.base) r.start_pos r.end_pos l h0 h1
